theories/ftlr/Lea.v
@@ -29,7 +29,7 @@ Section fundamental.
       apply elem_of_dom. apply lookup_insert_is_Some'; eauto. }
 
     iIntros "!>" (regs' retv). iDestruct 1 as (HSpec) "[Ha Hmap]".
-    destruct HSpec as [ * Hdst ? Hz Hoffset HincrPC | * Hdst Hz Hoffset HincrPC | ].
+    destruct HSpec as [ * Hdst Hz Hoffset HincrPC | * Hdst Hz Hoffset HincrPC | ].
     { apply incrementPC_Some_inv in HincrPC as (p''&b''&e''&a''& ? & HPC & Z & Hregs').
 
       assert (p'' = p ∧ b'' = b ∧ e'' = e) as (-> & -> & ->).
@@ -56,7 +56,6 @@ Section fundamental.
       { subst regs'. rewrite insert_insert. iApply "Hmap". }
       iModIntro.
       iApply (interp_weakening with "IH Hinv"); auto; try solve_addr.
-      { destruct Hp; by subst p. }
       { by rewrite PermFlowsToReflexive. } }
     { apply incrementPC_Some_inv in HincrPC as (p''&b''&e''&a''& ? & HPC & Z & Hregs').
 
@@ -84,7 +83,6 @@ Section fundamental.
       { subst regs'. rewrite insert_insert. iApply "Hmap". }
       iModIntro.
       iApply (interp_weakening with "IH Hinv"); auto; try solve_addr.
-      { destruct Hp; by subst p. }
       { by rewrite PermFlowsToReflexive. } }
     { iApply wp_pure_step_later; auto.
       iMod ("Hcls" with "[HP Ha]");[iExists w;iFrame|iModIntro].
