theories/proofmode/contiguous.v
@@ -322,14 +322,14 @@ Proof.
   inversion HH; auto.
 Qed.
 
-Lemma isCorrectPC_range_perm_non_E p b e a0 an :
-  isCorrectPC_range p b e a0 an →
-  (a0 < an)%a →
-  p ≠ E.
-Proof.
-  intros HH1 HH2. pose proof (isCorrectPC_range_perm _ _ _ _ _ HH1 HH2).
-  naive_solver.
-Qed.
+(* Lemma isCorrectPC_range_perm_non_E p b e a0 an : *)
+(*   isCorrectPC_range p b e a0 an → *)
+(*   (a0 < an)%a → *)
+(*   p ≠ E. *)
+(* Proof. *)
+(*   intros HH1 HH2. pose proof (isCorrectPC_range_perm _ _ _ _ _ HH1 HH2). *)
+(*   naive_solver. *)
+(* Qed. *)
 
 Lemma isCorrectPC_range_restrict p b e a0 an a0' an' :
   isCorrectPC_range p b e a0 an →
