theories/rules/rules_Lea.v
@@ -54,7 +54,6 @@ Section cap_lang_rules.
   :=
   | Lea_spec_success_cap: forall p b e a z a',
     regs !! r1 = Some (WCap p b e a) ->
-    p ≠ E ->
     z_of_argument regs rv = Some z ->
     (a + z)%a = Some a' ->
     incrementPC
@@ -120,9 +119,7 @@ Section cap_lang_rules.
        unfold is_mutable_range in Hr1v.
        assert (c = Failed ∧ σ2 = (r, m)) as (-> & ->).
        { destruct r1v as [ | [p b e a | ] | ]; try by inversion Hr1v.
-         all: try by simplify_pair_eq.
-         destruct p; try congruence.
-         simplify_pair_eq; auto. }
+         all: try by simplify_pair_eq. }
        iFailWP "Hφ" Lea_fail_allowed. }
 
      (* Now the proof splits depending on the type of value in r1v *)
@@ -130,10 +127,7 @@ Section cap_lang_rules.
      1,4: inversion Hr1v.
 
      (* First, the case where r1v is a capability *)
-     + destruct (perm_eq_dec p E); [ subst p |].
-       { rewrite /is_mutable_range in Hr1v; congruence. }
-
-       destruct (a + argz)%a as [ a' |] eqn:Hoffset; cycle 1.
+     + destruct (a + argz)%a as [ a' |] eqn:Hoffset; cycle 1.
        { (* Failure: offset is too large *)
          assert (c = Failed ∧ σ2 = (r, m)) as (-> & ->)
              by (destruct p; inversion Hstep; auto).
@@ -158,7 +152,7 @@ Section cap_lang_rules.
        eapply updatePC_success_incl in HuPC. 2: by eapply insert_mono; eauto.
        rewrite HuPC in Hstep; clear HuPC.
        eassert ((c, σ2) = (NextI, _)) as HH.
-       { destruct p; cbn in Hstep; eauto. congruence. }
+       { destruct p; cbn in Hstep; eauto. }
        simplify_pair_eq.
 
        iFrame.
@@ -208,7 +202,6 @@ Section cap_lang_rules.
      isCorrectPC (WCap pc_p pc_b pc_e pc_a) →
      (a' + 1)%a = Some pc_a' →
      (pc_a + z)%a = Some a' →
-     pc_p ≠ E →
 
      {{{ ▷ PC ↦ᵣ WCap pc_p pc_b pc_e pc_a
            ∗ ▷ pc_a ↦ₐ w
@@ -219,7 +212,7 @@ Section cap_lang_rules.
               ∗ pc_a ↦ₐ w
               ∗ rv ↦ᵣ WInt z }}}.
    Proof.
-     iIntros (Hinstr Hvpc Hpca' Ha' Hnep φ) "(>HPC & >Hpc_a & >Hrv) Hφ".
+     iIntros (Hinstr Hvpc Hpca' Ha' φ) "(>HPC & >Hpc_a & >Hrv) Hφ".
      iDestruct (map_of_regs_2 with "HPC Hrv") as "[Hmap %]".
      iApply (wp_lea with "[$Hmap Hpc_a]"); eauto; simplify_map_eq; eauto.
      by rewrite !dom_insert; set_solver+.
@@ -235,8 +228,7 @@ Section cap_lang_rules.
        simplify_map_eq. }
      { (* Failure (contradiction) *)
        destruct Hfail; try incrementPC_inv; simplify_map_eq; eauto.
-       destruct pc_p; congruence.
-       congruence.
+       destruct p; congruence.
      }
     Unshelve. all: auto.
    Qed.
@@ -246,7 +238,6 @@ Section cap_lang_rules.
      isCorrectPC (WCap pc_p pc_b pc_e pc_a) →
      (pc_a + 1)%a = Some pc_a' →
      (a + z)%a = Some a' →
-     p ≠ E →
 
      {{{ ▷ PC ↦ᵣ WCap pc_p pc_b pc_e pc_a
            ∗ ▷ pc_a ↦ₐ w
@@ -259,7 +250,7 @@ Section cap_lang_rules.
               ∗ rv ↦ᵣ WInt z
               ∗ r1 ↦ᵣ WCap p b e a' }}}.
    Proof.
-     iIntros (Hinstr Hvpc Hpca' Ha' Hnep ϕ) "(>HPC & >Hpc_a & >Hr1 & >Hrv) Hφ".
+     iIntros (Hinstr Hvpc Hpca' Ha' ϕ) "(>HPC & >Hpc_a & >Hr1 & >Hrv) Hφ".
      iDestruct (map_of_regs_3 with "HPC Hrv Hr1") as "[Hmap (%&%&%)]".
      iApply (wp_lea with "[$Hmap Hpc_a]"); eauto; simplify_map_eq; eauto.
      by rewrite !dom_insert; set_solver+.
@@ -277,8 +268,7 @@ Section cap_lang_rules.
        simplify_map_eq. }
      { (* Failure (contradiction) *)
        destruct Hfail; try incrementPC_inv; simplify_map_eq; eauto.
-       destruct p; congruence.
-       congruence.
+       destruct pc_p; congruence.
      }
     Unshelve. all: auto.
    Qed.
@@ -288,7 +278,6 @@ Section cap_lang_rules.
      isCorrectPC (WCap pc_p pc_b pc_e pc_a) →
      (a' + 1)%a = Some pc_a' →
      (pc_a + z)%a = Some a' →
-     pc_p ≠ E →
 
      {{{ ▷ PC ↦ᵣ WCap pc_p pc_b pc_e pc_a
            ∗ ▷ pc_a ↦ₐ w }}}
@@ -297,7 +286,7 @@ Section cap_lang_rules.
          PC ↦ᵣ WCap pc_p pc_b pc_e pc_a'
             ∗ pc_a ↦ₐ w }}}.
    Proof.
-     iIntros (Hinstr Hvpc Hpca' Ha' Hnep ϕ) "(>HPC & >Hpc_a) Hφ".
+     iIntros (Hinstr Hvpc Hpca' Ha' ϕ) "(>HPC & >Hpc_a) Hφ".
      iDestruct (map_of_regs_1 with "HPC") as "Hmap".
      iApply (wp_lea with "[$Hmap Hpc_a]"); eauto; simplify_map_eq; eauto.
      iNext. iIntros (regs' retv) "(#Hspec & Hpc_a & Hmap)".
@@ -311,8 +300,7 @@ Section cap_lang_rules.
        simplify_map_eq. }
      { (* Failure (contradiction) *)
        destruct Hfail; try incrementPC_inv; simplify_map_eq; eauto.
-       destruct pc_p; congruence.
-       congruence.
+       destruct p; congruence.
      }
      Unshelve. all: auto.
    Qed.
@@ -322,7 +310,6 @@ Section cap_lang_rules.
      isCorrectPC (WCap pc_p pc_b pc_e pc_a) →
      (pc_a + 1)%a = Some pc_a' →
      (a + z)%a = Some a' →
-     p ≠ E →
 
      {{{ ▷ PC ↦ᵣ WCap pc_p pc_b pc_e pc_a
            ∗ ▷ pc_a ↦ₐ w
@@ -333,7 +320,7 @@ Section cap_lang_rules.
             ∗ pc_a ↦ₐ w
             ∗ r1 ↦ᵣ WCap p b e a' }}}.
    Proof.
-     iIntros (Hinstr Hvpc Hpca' Ha' Hnep ϕ) "(>HPC & >Hpc_a & >Hr1) Hφ".
+     iIntros (Hinstr Hvpc Hpca' Ha' ϕ) "(>HPC & >Hpc_a & >Hr1) Hφ".
      iDestruct (map_of_regs_2 with "HPC Hr1") as "[Hmap %]".
      iApply (wp_lea with "[$Hmap Hpc_a]"); eauto; simplify_map_eq; eauto.
      by rewrite !dom_insert; set_solver+.
@@ -350,8 +337,7 @@ Section cap_lang_rules.
        simplify_map_eq. }
      { (* Failure (contradiction) *)
        destruct Hfail; try incrementPC_inv; simplify_map_eq; eauto.
-       destruct p; congruence.
-       congruence.
+       destruct pc_p; congruence.
      }
      Unshelve. all:auto.
    Qed.
